## Problem 1
	- Let \(\Delta(a) = Q(s, a) - Q^{\prime}(s, a)\) for \(a \in \mathcal{A}\).
	- ### Part 1
		- Let:
		  \[
		  M = \max_{a \in \mathcal{A}} Q(s, a), \quad M' = \max_{a' \in \mathcal{A}} Q^{\prime}(s, a').
		  \]
		  For any \(a \in \mathcal{A}\):
		  \[
		  M \geq Q(s, a) \quad \text{and} \quad M' \leq Q^{\prime}(s, a) + \max_{a \in \mathcal{A}} |Q(s, a) - Q^{\prime}(s, a)|
		  \]
		  \[
		  M - M' \leq Q(s, a) - (Q^{\prime}(s, a) - \max_{a \in \mathcal{A}} |Q(s, a) - Q^{\prime}(s, a)|) \leq \max_{a \in \mathcal{A}} |Q(s, a) - Q^{\prime}(s, a)|.
		  \]
		  \[
		  M' - M \leq \max_{a \in \mathcal{A}} |Q(s, a) - Q^{\prime}(s, a)|
		  \]
		  \[
		  \left|M - M'\right| \leq \max_{a \in \mathcal{A}} |Q(s, a) - Q^{\prime}(s, a)|,
		  \]
	- ### Part 2
		- Let:
		  \[
		  m = \min_{a \in \mathcal{A}} Q(s, a), \quad m' = \min_{a' \in \mathcal{A}} Q^{\prime}(s, a').
		  \]
		  \[
		  m \leq Q(s, a) \quad \text{and} \quad m' \geq Q^{\prime}(s, a) - \max_{a \in \mathcal{A}} |Q(s, a) - Q^{\prime}(s, a)|.
		  \]
		  \[
		  m - m' \leq \max_{a \in \mathcal{A}} |Q(s, a) - Q^{\prime}(s, a)|.
		  \]
		  \[
		  m' - m \leq \max_{a \in \mathcal{A}} |Q(s, a) - Q^{\prime}(s, a)|.
		  \]
		  \[
		  \left|m - m'\right| \leq \max_{a \in \mathcal{A}} |Q(s, a) - Q^{\prime}(s, a)|,
		  \]
	- ### Part 3
		- Let:
		  \[
		  \bar{Q} = \frac{1}{|\mathcal{A}|} \sum_{a \in \mathcal{A}} Q(s, a), \quad \bar{Q}' = \frac{1}{|\mathcal{A}|} \sum_{a' \in \mathcal{A}} Q^{\prime}(s, a').
		  \]
		  \[
		  \left| \bar{Q} - \bar{Q}' \right| = \left| \frac{1}{|\mathcal{A}|} \sum_{a \in \mathcal{A}} (Q(s, a) - Q^{\prime}(s, a)) \right|.
		  \]
		- By the triangle inequality:
		  \[
		  \left| \bar{Q} - \bar{Q}' \right| \leq \frac{1}{|\mathcal{A}|} \sum_{a \in \mathcal{A}} \left| Q(s, a) - Q^{\prime}(s, a) \right| \leq \max_{a \in \mathcal{A}} \left| Q(s, a) - Q^{\prime}(s, a) \right|,
		  \]
	- ### Part 4
		- Let:
		  \[
		  Z = \frac{1}{|\mathcal{A}|} \sum_{a \in \mathcal{A}} \exp(\omega Q(s, a)), \quad Z' = \frac{1}{|\mathcal{A}|} \sum_{a' \in \mathcal{A}} \exp(\omega Q^{\prime}(s, a')).
		  \]
		  \[
		  \left| \log Z - \log Z' \right| = \left| \log \left( \frac{Z}{Z'} \right) \right| \leq \left| \frac{Z - Z'}{Z'} \right|
		  \]
		  \[
		  Z - Z' = \frac{1}{|\mathcal{A}|} \sum_{a \in \mathcal{A}} \left( \exp(\omega Q(s, a)) - \exp(\omega Q^{\prime}(s, a)) \right).
		  \]
		- Using the first-order Taylor expansion around \(Q^{\prime}(s, a)\):
		  \[
		  \exp(\omega Q(s, a)) \approx \exp(\omega Q^{\prime}(s, a)) \left( 1 + \omega \Delta(a) + O(\Delta(a)^2) \right),
		  \]
		  \[
		  Z \approx Z' + \frac{\omega}{|\mathcal{A}|} \sum_{a \in \mathcal{A}} \Delta(a) \exp(\omega Q^{\prime}(s, a)).
		  \]
		  \[
		  \left|Z - Z'\right| \leq \max_{a \in \mathcal{A}} \left|Q(s, a) - Q^{\prime}(s, a)\right| \cdot C,
		  \]
		- Since \(\frac{Z - Z'}{Z'}\) is bounded by the maximum difference
		  \[
		  \left| \log Z - \log Z' \right| \leq \max_{a \in \mathcal{A}} |Q(s, a) - Q^{\prime}(s, a)|,
		  \]
		  and dividing by \(\omega\) completes the proof.
- ## Problem 2
	- ### Part 1
		- The optimal value function \(V^*\) for \(\mathcal{M}\) satisfies the Bellman equation:
		  \[
		  V^*(s) = \max_{a \in \mathcal{A}} \left( r(s, a) + \gamma \sum_{s' \in \mathcal{S}} P_{\mathcal{T}}(s' | s, a) V^*(s') \right).
		  \]
		  Similarly, the optimal value function \(\hat{V}^*\) for \(\hat{\mathcal{M}}\) satisfies:
		  \[
		  \hat{V}^*(s) = \max_{a \in \mathcal{A}} \left( \hat{r}(s, a) + \gamma \sum_{s' \in \mathcal{S}} P_{\mathcal{T}}(s' | s, a) \hat{V}^*(s') \right).
		  \]
		  Since \(|\hat{r}(s, a) - r(s, a)| \leq \epsilon\),
		  \[
		  \hat{V}^*(s) \leq \max_{a \in \mathcal{A}} \left( r(s, a) + \epsilon + \gamma \sum_{s' \in \mathcal{S}} P_{\mathcal{T}}(s' | s, a) \hat{V}^*(s') \right).
		  \]
		  \[
		  \hat{V}^*(s) \leq V^*(s) + \epsilon + \gamma \sum_{s' \in \mathcal{S}} P_{\mathcal{T}}(s' | s, a) \hat{V}^*(s').
		  \]
		  \[
		  \hat{V}^*(s) \leq V^*(s) + \epsilon + \gamma \hat{V}^*(s),
		  \]
		  \[
		  \hat{V}^*(s) (1 - \gamma) \leq V^*(s) + \epsilon.
		  \]
		  \[
		  \hat{V}^*(s) \leq \frac{V^*(s) + \epsilon}{1 - \gamma}.
		  \]
		  \[
		  V^*(s) - \hat{V}^*(s) \geq \frac{V^*(s) - \epsilon}{1 - \gamma}.
		  \]
		  \[
		  V^*(s) - \hat{V}^*(s) \leq \epsilon \cdot \frac{1}{1 - \gamma},
		  \]
		  and since this holds for all states \(s \in \mathcal{S}\), we conclude:
		  \[
		  V^* - \hat{V}^* \leq \frac{\epsilon}{1 - \gamma}.
		  \]
	- ### Part 2
		- An alternative definition of \(\hat{r}\):
		  \[
		  \hat{r}(s, a) = r(s, a) + \epsilon.
		  \]
		  Using the Bellman equation for \(\hat{V}^*\):
		  \[
		  \hat{V}^*(s) = \max_{a \in \mathcal{A}} \left( r(s, a) + \epsilon + \gamma \sum_{s' \in \mathcal{S}} P_{\mathcal{T}}(s' | s, a) \hat{V}^*(s') \right).
		  \]
		  \[
		  \hat{V}^*(s) = \max_{a \in \mathcal{A}} \left( r(s, a) + \gamma \sum_{s' \in \mathcal{S}} P_{\mathcal{T}}(s' | s, a) \hat{V}^*(s') \right) + \epsilon.
		  \]
		  \[
		  \hat{V}^*(s) = V^*(s) + \epsilon.
		  \]
		  \[
		  \hat{V}^* = V^* + \epsilon.
		  \]
		  
		  1. \(V^* - \hat{V}^* \leq \frac{\epsilon}{1 - \gamma}\).
		  2. \(\hat{V}^* = V^* + \epsilon\).
- ## Problem 3
	- 1. **At \(t=1\)**:
		- \(A_1 = 1\), \(R_1 = 1\)
		- Action 1 is chosen. Since it's the first action and the estimates are all equal, this could be **possible** exploratory.
	- 2. **At \(t=2\)**:
		- \(A_2 = 2\), \(R_2 = 1\)
		- Action 2 is chosen. The only information so far is from action 1. This is **definitely** exploratory.
	- 3. **At \(t=3\)**:
		- \(A_3 = 2\), \(R_3 = 2\)
		- Action 2 is selected again, and now we have more evidence about arm 2's performance. Given that it was chosen again, it suggests that it may be the best so far. This action is **possible** exploratory.
	- 4. **At \(t=4\)**:
		- \(A_4 = 2\), \(R_4 = 2\)
		- Again, action 2 is chosen. The estimate for arm 2 will continue to increase based on the rewards received. This is **possible** exploratory.
	- 5. **At \(t=5\)**:
		- \(A_5 = 3\), \(R_5 = 0\)
		- Here, action 3 is chosen. Given that arm 2 has performed well, choosing arm 3 at this point is **definitely** exploratory
	- | time seep | $\hat{\mu}_1$ | $\widehat{\mu}_2$ | $\hat{\mu}_3$ | $\widehat{\mu}_4$ | $\operatorname{action}$ | $r$ |
	  | :---: | :---: | :---: | :---: | :---: | :---: | :---: |
	  | 1 | 0 | 0 | 0 | 0 | 1 | 1 |
	  | 2 | 1 | 0 | 0 | 0 | 2 | 1 |
	  | 3 | 1 | 1 | 0 | 0 | 2 | 2 |
	  | 4 | 1 | 1.5 | 0 | 0 | 2 | 2 |
	  | 5 | 1 | $\frac{5}{3}$ | 0 | 0 | 3 | 3 |
	- According to the table above.
	  The Definitely exploratory: $A_2, A_5$
	  The possible exploratory: $A_1, A_3, A_4$.
- ## Problem 4
	- ### Part 1
		- According to lecture notes,
		  $\begin{aligned} \overline{R_T} & \leqslant \Delta\left(k+T \exp \left(-\frac{k}{4} \Delta^2\right)\right) \\ & =\Delta k+T \Delta \exp \left(-\frac{k}{4} \Delta^2\right) \\ & \leqslant \Delta k+T \max _{\Delta>_0} \Delta \exp \left(-\frac{k}{4} \Delta^2\right)\end{aligned}$
		- let  $f(X)=X \exp \left(-\frac{k}{4} X^2\right)$
		  $X$ $f^{\prime}(X)=\exp \left(-\frac{k}{4} X^2\right)-\frac{k}{2} X^2 \exp \left(-\frac{k}{4} X^2\right)$
		  let $f^{\prime}(X)=0$, so $f(X)$ reach maximum when $X^*=\sqrt{\frac{2}{k}}$
		  Hence, $\overline{R_T} \leq \Delta K+T \sqrt{\frac{2}{k}} \exp \left(-\frac{1}{2}\right)$
		  since $k$ is dependent on $T$ bur independent of $\Delta$, we can select $k=T^{\frac{2}{3}}$,
		  then $\overline{R_T} \leqslant \Delta T^{\frac{2}{3}}+\sqrt{2} \exp \left(-\frac{1}{2}\right) T^{\frac{2}{3}}=\left(\Delta+\sqrt{2} \exp \left(-\frac{1}{2}\right)\right) T^{\frac{2}{3}}$
		- Therefore, there exists a constant $C>0$ that $\overline{R_T} \leqslant(\Delta+C) T^{2 / 3}$.
	- ### Part 2
		- 1. if $\Delta \leq \frac{1}{\sqrt{n}}$, $R_n \leq n \Delta$. => $R_n \leq \sqrt{n}$
		  2. if $\Delta>\frac{1}{\sqrt{n}}$, then $R_n \leqslant \Delta+\frac{4}{\Delta}\left(1+\max \left\{0, \log \left(\frac{n \Delta^2}{4}\right)\right\}\right)<\Delta+4 \sqrt{n}+\max _{\Delta>0}\left\{0, \frac{4}{\Delta} \log \left(\frac{n \Delta^2}{4}\right)\right\} \text {. }$
		- let $f(X)=\frac{4}{X} \log \left(\frac{k X^2}{4}\right)$
		  $f^{\prime}(X)=-\frac{4}{X^2} \log \left(\frac{n X^2}{4}\right)+\frac{8}{X^2}$.
		  So $f(X)$ reach maximum when $X^*=\frac{2 e^1}{\sqrt{n}}>$
		  Therefore, $R_n<\Delta+4 \sqrt{n}+4 e^{-1} \sqrt{n}=\Delta+\left(4+4 e^{-1}\right) \sqrt{n}$
		- (1),(2) => $R_n \leqslant \Delta+C \sqrt{n}$ where $C>0$
-
-